src/computational_monads/simulation_semantics/constructions/logging/seeded_oracle.lean
@@ -3,9 +3,8 @@ Copyright (c) 2022 Devon Tuma. All rights reserved.
 Released under Apache 2.0 license as described in the file LICENSE.
 Authors: Devon Tuma
 -/
-import computational_monads.simulation_semantics.constructions.logging.logging_oracle
-import computational_monads.query_tracking.query_log.fork
-import computational_monads.query_tracking.query_log.lookup
+import computational_monads.query_tracking.query_seed.generate_seed
+import computational_monads.simulation_semantics.oracle_compose
 
 /-!
 # Seeded Simulation Oracle
@@ -29,57 +28,13 @@ variables {spec spec' spec'' : oracle_spec} {α β γ : Type}
 /-- Use the first element of the `seed` as the query result if inputs match.
   If the query values don't match then throw away the seed as computation has diverged.
   Using this with a log from a previous computation ensures they behave identically. -/
-def seeded_oracle (spec : oracle_spec) :
-  sim_oracle spec spec (query_log spec) :=
-{ default_state := query_log.init spec,
-  o := λ i ⟨t, seed⟩, match seed.lookup_fst i t with
-    -- Once the seed is empty, just keep it empty going forward
-    | none := (λ u, (u, query_log.init spec)) <$> query i t
-    | (some u) := return (u, seed.remove_head i)
-    end }
+def seeded_oracle {spec : oracle_spec} : sim_oracle spec spec (query_seed spec) :=
+{ o := λ i x, query_seed.get_or_else x.2 i x.1,
+  default_state := ∅ }
 
 namespace seeded_oracle
 
-variables (log : query_log spec) (log' : query_log spec')
-
-section simulate
-
-
-end simulate
-
-section eval_dist
-
--- Log and run, run from seed, return original output -> looks like just logging
-lemma eval_dist_seeded_oracle_fst (oa : oracle_comp spec α) (i : spec.ι)
-  (choose_fork : α → query_log spec → option ℕ) :
-⁅do{ ⟨a, log⟩ ← simulate (logging_oracle spec) oa (query_log.init spec),
-      seed ← return (log.fork_cache i $ choose_fork a log).to_seed,
-      ⟨a', log'⟩ ← simulate (seeded_oracle spec) oa seed,
-      return (a, log) }⁆ =
-  ⁅(simulate (logging_oracle spec) oa (query_log.init spec))⁆ :=
-sorry
-
--- Log and run, run from seed, return new output -> looks like just logging
-lemma eval_dist_seeded_oracle_snd (oa : oracle_comp spec α) (i : spec.ι)
-  (choose_fork : α → query_log spec → option ℕ) :
-⁅do{ ⟨a, log⟩ ← simulate (logging_oracle spec) oa (query_log.init spec),
-      seed ← return (log.fork_cache i $ choose_fork a log).to_seed,
-      ⟨a', log'⟩ ← simulate (seeded_oracle spec) oa (seed),
-      return (a', log') }⁆ =
-  ⁅(simulate (logging_oracle spec) oa (query_log.init spec))⁆ :=
-sorry
-
--- The log values match up until the point where the log was forked
-lemma seeded_oracle_log_eq_log (oa : oracle_comp spec α) (i : spec.ι)
-  (choose_fork : α → query_log spec → option ℕ) :
-do{ ⟨a, log⟩ ← simulate (logging_oracle spec) oa (query_log.init spec),
-    seed ← return (log.fork_cache i $ choose_fork a log).to_seed,
-    ⟨a', log'⟩ ← simulate (seeded_oracle spec) oa (seed),
-    return (a, log, log') }.support
-  ⊆ λ ⟨a, log, log'⟩, log.fork_cache i (choose_fork a log) =
-      log'.fork_cache i (choose_fork a log) :=
-sorry
-
-end eval_dist
+@[simp] lemma seeded_oracle_apply (i : spec.ι) (x : spec.domain i × query_seed spec) :
+  seeded_oracle i x = query_seed.get_or_else x.2 i x.1 := rfl
 
 end seeded_oracle
