src/computational_monads/constructions/fork.lean
@@ -1,0 +1,178 @@
+/-
+Copyright (c) 2023 Devon Tuma. All rights reserved.
+Released under Apache 2.0 license as described in the file LICENSE.
+Authors: Devon Tuma
+-/
+import computational_monads.simulation_semantics.constructions.logging.seeded_oracle
+import computational_monads.simulation_semantics.constructions.logging.logging_oracle
+import computational_monads.query_tracking.query_log.basic
+import computational_monads.coercions.instances
+import computational_monads.simulation_semantics.oracle_compose
+
+/-!
+# Forking Computations at a Query
+-/
+
+open oracle_spec
+
+variables {α β γ : Type} {spec : oracle_spec} {i : spec.ι} {q : ℕ}
+
+namespace oracle_comp
+
+section sec_adversary
+
+structure sec_adversary (spec : oracle_spec) (α : Type) :=
+(run : oracle_comp (uniform_selecting ++ spec) α)
+(qb : oracle_comp.query_count (uniform_selecting ++ spec))
+
+end sec_adversary
+
+end oracle_comp
+
+
+section forking_adversary
+
+open oracle_comp
+
+structure forking_adversary (α : Type) (i : spec.ι) (q : ℕ)
+  extends sec_adversary spec α :=
+(choose_fork : α → option (fin q.succ))
+(q_eq_bound : qb (sum.inr i) = q)
+
+def forking_adversary.success (adv : forking_adversary α i q) : α → Prop :=
+λ x, adv.choose_fork x ≠ none
+
+section fork_result
+
+structure fork_result (adv : forking_adversary α i q) :=
+(chosen_fork : option (fin q.succ))
+(side_output₁ side_output₂ : α)
+(seed₁ seed₂ : query_seed (uniform_selecting ++ spec))
+
+variable {adv : forking_adversary α i q}
+
+@[inline, reducible] def fork_result.get_cf (x : fork_result adv) :
+  fin (q.succ) := x.chosen_fork.get_or_else 0
+
+def fork_success (x : fork_result adv) : Prop :=
+match x.chosen_fork with
+| none := false
+| (some cf) := query_seed.seed_differs x.seed₁ x.seed₂ (sum.inr i) cf
+end
+
+end fork_result
+
+namespace forking_adversary
+
+section of_choose_input
+
+def of_choose_input (adv : sec_adversary spec α) (choose_input : α → spec.domain i) :
+  forking_adversary (α × query_log (uniform_selecting ++ spec)) i (adv.qb (sum.inr i)) :=
+{ run := simulate logging_oracle adv.run ∅,
+  choose_fork := λ z, begin
+    have inp := choose_input z.1,
+    have ts : list (spec.domain i) := (z.2 (sum.inr i)).map prod.fst,
+    exact if inp ∈ ts then some ↑(list.index_of inp ts) else none,
+  end,
+  qb := adv.qb,
+  q_eq_bound := rfl
+}
+
+end of_choose_input
+
+@[inline, reducible] def fresh_query_count (adversary : forking_adversary α i q)
+  (fp : fin q.succ) : query_count (uniform_selecting ++ spec) :=
+query_count.of_nat (sum.inr i) (q - fp)
+
+@[inline, reducible] noncomputable def shared_query_count (adversary : forking_adversary α i q)
+  (fp : fin q.succ) : query_count (uniform_selecting ++ spec) :=
+adversary.qb - fresh_query_count adversary fp
+
+end forking_adversary
+
+end forking_adversary
+
+namespace oracle_comp
+
+/-- Fork a `forking_adversary` at the point defined by `cf`. -/
+noncomputable def fork (adversary : forking_adversary α i q) :
+  oracle_comp (uniform_selecting ++ spec) (fork_result adversary) :=
+let i' : (uniform_selecting ++ spec).ι := sum.inr i in
+do {
+  -- Generate an initial seed with enouch values to reach the adversary's query bound.
+  seed ← generate_seed adversary.qb,
+  z₁ ← simulate' seeded_oracle adversary.run seed,
+  fp₁ ← return ((adversary.choose_fork z₁).get_or_else 0),
+  -- Regenerate seed values after the chosen forking point.
+  shared_seed ← return (seed.take_queries i' fp₁),
+  fresh_seed ← generate_seed (adversary.fresh_query_count fp₁),
+  -- Run the adversary again using the new seeded values.
+  z₂ ← simulate' seeded_oracle adversary.run (shared_seed ++ fresh_seed),
+  fp₂ ← return ((adversary.choose_fork z₂).get_or_else 0),
+  -- Return the final result, assuming that both runs choose the same forking point
+  let success := (adversary.choose_fork z₁).is_some ∧ fp₁ = fp₂ ∧
+                    (seed i').nth (fp₁ + 1) ≠ (fresh_seed i').nth 0 in
+  return (fork_result.mk (if success then fp₁ else none) z₁ z₂ seed (shared_seed ++ fresh_seed))
+}
+
+variables (adversary : forking_adversary α i q) (fr : fork_result adversary)
+
+/-- Both the resulting `query_seed`s from running `fork` have the same number of seeded values. -/
+lemma to_query_count_seed_eq_to_query_count_seed (h : fr ∈ (fork adversary).support) :
+  fr.seed₁.to_query_count = fr.seed₂.to_query_count :=
+begin
+  sorry
+end
+
+/-- Up until the forking point, both resulting `query_seed`s have the same seed values. -/
+lemma take_queries_seed_eq_take_queries_seed (h : fr ∈ (fork adversary).support) :
+  (fr.seed₁.take_queries (sum.inr i) fr.get_cf) =
+    (fr.seed₁.take_queries (sum.inr i) fr.get_cf) :=
+begin
+  sorry
+end
+
+/-- The first side output is in the support of simulating the adversary with the first seed. -/
+lemma mem_support_simulate'_seed₁ (h : fr ∈ (fork adversary).support) :
+  fr.side_output₁ ∈ (simulate' seeded_oracle adversary.run fr.seed₁).support :=
+begin
+  sorry,
+end
+
+/-- The second side output is in the support of simulating the adversary with the second seed. -/
+lemma mem_support_simulate'_seed₂ (h : fr ∈ (fork adversary).support) :
+  fr.side_output₂ ∈ (simulate' seeded_oracle adversary.run fr.seed₂).support :=
+begin
+  sorry,
+end
+
+/-- If `fork` returns success then both runs chose the same fork value. -/
+lemma choose_fork_eq_of_fork_success (h : fr ∈ (fork adversary).support) (hfr : fork_success fr) :
+  adversary.choose_fork fr.side_output₁ = fr.chosen_fork ∧
+    adversary.choose_fork fr.side_output₂ = fr.chosen_fork :=
+begin
+  sorry
+end
+
+/-- If `fork` returns success then the adversary must have thrown away at least one value. -/
+lemma choose_fork_ne_of_fork_success (h : fr ∈ (fork adversary).support) (hfr : fork_success fr) :
+  fr.chosen_fork ≠ some q :=
+begin
+  sorry
+end
+
+/-- If `fork` returns success then the output after the forking point-/
+lemma seed_differs_of_fork_success (h : fr ∈ (fork adversary).support) (hfr : fork_success fr) :
+  (fr.seed₁ (sum.inr i)).nth (fr.get_cf + 1) ≠
+    (fr.seed₂ (sum.inr i)).nth (fr.get_cf + 1) :=
+begin
+  sorry
+end
+
+theorem prob_event_fork_success : ⁅fork_success | fork adversary⁆ ≥
+  ⁅(≠) none | adversary.choose_fork <$> adversary.run⁆ ^ 2 / q - (fintype.card (spec.range i))⁻¹ :=
+begin
+  sorry
+end
+
+end oracle_comp
