src/computational_monads/query_tracking/query_seed/get_or_else.lean
@@ -1,0 +1,43 @@
+/-
+Copyright (c) 2023 Devon Tuma. All rights reserved.
+Released under Apache 2.0 license as described in the file LICENSE.
+Authors: Devon Tuma
+-/
+import computational_monads.query_tracking.query_seed.basic
+import computational_monads.query_tracking.query_count.possible_outcomes
+import computational_monads.constructions.uniform_select
+
+/-!
+# Structure for Bounding Number of Queries Made by a Computation
+
+This file defines a function `generate_seed` that pre-computes a number of oracle outputs that can
+be used in a computation, choosing them all uniformly at random.
+The output is given by a `query_seed`, and the count is specified by a `query_count`.
+
+If the number of seeded values is higher than the specified count the values remain unchanged.
+The order in which the values are generated isn't specifically defined, as we use `finset.to_list`
+to determine the ordering, and so the definition is noncomputable.
+-/
+
+namespace oracle_comp
+
+open oracle_spec
+
+namespace query_seed
+
+variables {α β γ : Type} {spec : oracle_spec}
+
+def get_or_else (qs : query_seed spec) (i : spec.ι) (t : spec.domain i) :
+  oracle_comp spec (spec.range i × query_seed spec) :=
+match qs i with
+| [] := do {u ← query i t, return (u, qs)}
+| (u :: us) := return (u, qs.drop_queries i 1)
+end
+
+@[simp] lemma get_or_else_empty (i : spec.ι) (t : spec.domain i) :
+  get_or_else ∅ i t = do {u ← query i t, return (u, ∅)} :=
+by simp only [get_or_else, query_seed.empty_apply]
+
+end query_seed
+
+end oracle_comp
