src/computational_monads/simulation_semantics/constructions/tracking_oracle.lean
@@ -24,22 +24,15 @@ but this construction allows seperation of the components that affect state inde
 
 variables {α β γ : Type} {spec spec' spec'': oracle_spec}
 
+-- TODO: `is_stateless` seems more useful
 structure tracking_sim_oracle (spec spec' : oracle_spec) (S : Type)
   extends sim_oracle spec spec' S :=
-(default_state := default_state)
 (answer_query : Π (i : spec.ι), spec.domain i → oracle_comp spec' (spec.range i))
 (update_state : Π (s : S) (i : spec.ι), spec.domain i → spec.range i → S)
-(o := λ i x, (λ u, (u, update_state x.2 i x.1 u)) <$> (answer_query i x.1))
+(o_apply_eq : ∀ i x, o i x = (λ u, (u, update_state x.2 i x.1 u)) <$> (answer_query i x.1))
 
-structure stateless_sim_oracle (spec spec' : oracle_spec)
-  extends tracking_sim_oracle spec spec' unit :=
-(default_state := ())
-(answer_query := answer_query)
-(update_state := λ _ _ _ _, ())
-(o := λ i x, (λ u, (u, ())) <$> (answer_query i x.1))
-
-def identi_o (spec : oracle_spec) : stateless_sim_oracle spec spec :=
-{ answer_query := λ i t, oracle_comp.query i t }
+structure stateless_sim_oracle (spec spec' : oracle_spec) (S : Type)
+  extends tracking_sim_oracle spec spec' S, unique S
 
 /-- Oracle where the query result is indepenent of the current oracle state,
 although the new state may depend upon the previous state.
